theories/typing/uniq_bor.v
@@ -1,5 +1,5 @@
 From lrust.typing Require Export type.
-From lrust.typing Require Import type_context programs.
+From lrust.typing Require Import type_context programs mod_ty.
 Set Default Proof Using "Type".
 
 Implicit Type 𝔄 𝔅: syn_type.
@@ -32,7 +32,7 @@ Section uniq_bor.
     by iApply ty_shr_lft_mono.
   Qed.
   Next Obligation.
-    move=> 𝔄 ??? vπ *. have ?: Inhabited 𝔄 := populate (fst (vπ inhabitant)).
+    move=> 𝔄 ??? vπ *. have ?: Inhabited 𝔄 := populate (vπ inhabitant).1.
     iIntros "#LFT #? Bor κ'". iMod (bor_exists with "LFT Bor") as (vl) "Bor"; [done|].
     iMod (bor_sep with "LFT Bor") as "[BorMt Bor]"; [done|].
     iMod (bor_sep with "LFT Bor") as "[_ Bor]"; [done|].
@@ -136,7 +136,7 @@ Section typing.
   Proof.
     move=>/= ? vπ d ? vl ??. rewrite right_id. iIntros "#LFT PROPH [κ κ+] [In uniq]".
     case vl as [|[[]|][]]=>//. iDestruct "uniq" as (??[Le Eq]) "[Vo Bor]".
-    move: Le=> /succ_le[?[->Le]]. have ?: Inhabited 𝔄 := populate (fst (vπ inhabitant)).
+    move: Le=> /succ_le[?[->Le]]. have ?: Inhabited 𝔄 := populate (vπ inhabitant).1.
     iMod (bor_acc with "LFT Bor κ") as "[(%&%&(%& ↦ & ty)&⧖& Pc) ToBor]"; [solve_ndisj|].
     iIntros "/= !>!>!>". iMod (ty_own_proph with "LFT In ty κ+") as "Toξl";
     [solve_ndisj|]. iDestruct (uniq_agree with "Vo Pc") as %[<-->].
@@ -171,13 +171,52 @@ Section typing.
     eqtype E L (&uniq{κ} ty) (&uniq{κ} ty') id id.
   Proof. move=> [??][??]. by split; apply uniq_subtype. Qed.
 
+  Lemma read_uniq {𝔄} E L κ (ty: _ 𝔄):
+    Copy ty → lctx_lft_alive E L κ →
+    typed_read E L (&uniq{κ} ty) ty (&uniq{κ} ty) fst id.
+  Proof.
+    iIntros (? Alv vπ ?[[]|]??) "#LFT E Na L [In uniq] //".
+    have ?: Inhabited 𝔄 := populate (vπ inhabitant).1.
+    iDestruct "uniq" as (??[Le ?]) "[Vo Bor]". case d as [|]; [lia|].
+    iMod (Alv with "E L") as (?) "[κ ToL]"; [done|].
+    iMod (bor_acc with "LFT Bor κ") as
+      "[(%&%&(%& >↦ & #ty)& #>⧖ & Pc) ToBor]"; [done|].
+    iMod (uniq_strip_later with "Vo Pc") as (<-<-) "[Vo Pc]".
+    iDestruct (ty_size_eq with "ty") as "#>%". iIntros "!>".
+    iExists _, _, _. iSplit; [done|]. iFrame "↦ Na". iSplitR.
+    { iApply ty_own_depth_mono; [|done]. lia. }
+    iIntros "↦". iMod ("ToBor" with "[↦ Pc]") as "[? κ]".
+    { iNext. iExists _, _. iFrame "Pc ⧖". iExists _. by iFrame. }
+    iMod ("ToL" with "κ") as "$". iFrame "In". iExists _, _. by iFrame.
+  Qed.
+
+  Lemma write_uniq {𝔄} E L κ (ty: _ 𝔄):
+    lctx_lft_alive E L κ →
+    typed_write E L (&uniq{κ} ty) ty (&uniq{κ} ty) ty fst (λ v w, (w, v.2)).
+  Proof.
+    move=> Alv. split; [done|]. iIntros (vπ d[[]|]??) "#LFT #UNIQ E L [In uniq] //".
+    have ?: Inhabited 𝔄 := populate (vπ inhabitant).1.
+    iDestruct "uniq" as (??[Le ?]) "[Vo Bor]". move: Le=> /succ_le[?[->?]].
+    iMod (Alv with "E L") as (?) "[κ ToL]"; [done|].
+    iMod (bor_acc with "LFT Bor κ") as "[(%&%&(%& >↦ & ty)&_& Pc) ToBor]"; [done|].
+    iMod (uniq_strip_later with "Vo Pc") as (<-<-) "[Vo Pc]". iModIntro.
+    iExists _. iSplit; [done|]. iSplitL "↦ ty".
+    { iNext. iExists _. iFrame "↦". iApply ty_own_depth_mono; [|done]. lia. }
+    iIntros (wπ ?) "(% & >↦ & ty) #⧖ /=".
+    iMod (uniq_update with "UNIQ Vo Pc") as "[Vo Pc]"; [done|].
+    iMod ("ToBor" with "[↦ Pc ty]") as "[Bor κ]".
+    { iNext. iExists _, _. iFrame "⧖ Pc". iExists _. iFrame. }
+    iMod ("ToL" with "κ") as "$". iFrame "In". iExists _, _.
+    rewrite (proof_irrel (prval_to_inh' _) (prval_to_inh' vπ)). by iFrame.
+  Qed.
+
   Lemma tctx_reborrow_uniq {𝔄} E L p (ty: _ 𝔄) κ κ' :
     lctx_lft_incl E L κ' κ →
     tctx_incl E L +[p ◁ &uniq{κ} ty] +[p ◁ &uniq{κ'} ty; p ◁{κ'} &uniq{κ} ty]
       (λ post '-[(a, a')], ∀a'': 𝔄, post -[(a, a''); (a'', a')]).
   Proof.
     iIntros (κκ' ??[vπ[]]?) "#LFT #PROPH #UNIQ E L [p _] Obs".
-    have ?: Inhabited 𝔄 := populate (fst (vπ inhabitant)).
+    have ?: Inhabited 𝔄 := populate (vπ inhabitant).1.
     iDestruct (κκ' with "L E") as "#κ⊑κ'". iFrame "L".
     iDestruct "p" as ([[]|]??) "[⧖ [#In uniq]]"=>//.
     iDestruct "uniq" as (? ξi [Le Eq]) "[ξVo ξBor]". set ξ := PrVar _ ξi.
@@ -237,43 +276,39 @@ Section typing.
     by apply subtype_tctx_incl, uniq_subtype, eqtype_symm. } by move=>/= ?[[??]?].
   Qed.
 
-  Lemma read_uniq {𝔄} E L κ (ty: _ 𝔄):
-    Copy ty → lctx_lft_alive E L κ →
-    typed_read E L (&uniq{κ} ty) ty (&uniq{κ} ty) fst id.
-  Proof.
-    iIntros (? Alv vπ ?[[]|]??) "#LFT E Na L [In uniq] //".
-    have ?: Inhabited 𝔄 := populate (fst (vπ inhabitant)).
-    iDestruct "uniq" as (??[Le ?]) "[Vo Bor]". case d as [|]; [lia|].
-    iMod (Alv with "E L") as (?) "[κ ToL]"; [done|].
-    iMod (bor_acc with "LFT Bor κ") as
-      "[(%&%&(%& >↦ & #ty)& #>⧖ & Pc) ToBor]"; [done|].
-    iMod (uniq_strip_later with "Vo Pc") as (<-<-) "[Vo Pc]".
-    iDestruct (ty_size_eq with "ty") as "#>%". iIntros "!>".
-    iExists _, _, _. iSplit; [done|]. iFrame "↦ Na". iSplitR.
-    { iApply ty_own_depth_mono; [|done]. lia. }
-    iIntros "↦". iMod ("ToBor" with "[↦ Pc]") as "[? κ]".
-    { iNext. iExists _, _. iFrame "Pc ⧖". iExists _. by iFrame. }
-    iMod ("ToL" with "κ") as "$". iFrame "In". iExists _, _. by iFrame.
-  Qed.
-
-  Lemma write_uniq {𝔄} E L κ (ty: _ 𝔄):
+  Lemma tctx_uniq_mod_ty_out {𝔄 𝔅 ℭl} f g `{!@SemiIso 𝔄 𝔅 f g} κ ty (T: _ ℭl) p E L :
     lctx_lft_alive E L κ →
-    typed_write E L (&uniq{κ} ty) ty (&uniq{κ} ty) ty fst (λ v w, (w, v.2)).
+    tctx_incl E L (p ◁ &uniq{κ} (<{f}> ty) +:: T) (p ◁ &uniq{κ} ty +:: T)
+      (λ post '((b, b') -:: cl), post ((g b, g b') -:: cl)).
   Proof.
-    move=> Alv. split; [done|]. iIntros (vπ d[[]|]??) "#LFT #UNIQ E L [In uniq] //".
-    have ?: Inhabited 𝔄 := populate (fst (vπ inhabitant)).
-    iDestruct "uniq" as (??[Le ?]) "[Vo Bor]". move: Le=> /succ_le[?[->?]].
+    iIntros (Alv ??[vπ ?]?) "LFT #PROPH UNIQ E L /=[p T] Obs".
     iMod (Alv with "E L") as (?) "[κ ToL]"; [done|].
-    iMod (bor_acc with "LFT Bor κ") as "[(%&%&(%& >↦ & ty)&_& Pc) ToBor]"; [done|].
-    iMod (uniq_strip_later with "Vo Pc") as (<-<-) "[Vo Pc]". iModIntro.
-    iExists _. iSplit; [done|]. iSplitL "↦ ty".
-    { iNext. iExists _. iFrame "↦". iApply ty_own_depth_mono; [|done]. lia. }
-    iIntros (wπ ?) "(% & >↦ & ty) #⧖ /=".
-    iMod (uniq_update with "UNIQ Vo Pc") as "[Vo Pc]"; [done|].
-    iMod ("ToBor" with "[↦ Pc ty]") as "[Bor κ]".
-    { iNext. iExists _, _. iFrame "⧖ Pc". iExists _. iFrame. }
-    iMod ("ToL" with "κ") as "$". iFrame "In". iExists _, _.
-    rewrite (proof_irrel (prval_to_inh' _) (prval_to_inh' vπ)). by iFrame.
+    have ?: Inhabited 𝔅 := populate (vπ inhabitant).1.
+    have ?: Inhabited 𝔄 := populate (g inhabitant). set aπ := g ∘ fst ∘ vπ.
+    iDestruct "p" as ([[]|]? Ev) "[_ [In uniq]]"=>//.
+    iDestruct "uniq" as (? ξi [? Eq]) "[ξVo Bor]".
+    move: Eq. (set ξ := PrVar _ ξi)=> Eq.
+    iMod (bor_acc_cons with "LFT Bor κ") as "[(%&%& ↦ty & >#⧖ & ξPc) ToBor]"; [done|].
+    iMod (uniq_strip_later with "ξVo ξPc") as (<-<-) "[ξVo ξPc]".
+    iMod (uniq_intro aπ with "PROPH UNIQ") as (ζi) "[ζVo ζPc]"; [done|].
+    set ζ := PrVar _ ζi. iDestruct (uniq_proph_tok with "ζVo ζPc") as "(ζVo & ζ & ζPc)".
+    iMod (uniq_preresolve ξ [ζ] (λ π, f (π ζ)) with "PROPH ξVo ξPc [$ζ]") as
+    "(Obs' & [ζ _] & ToξPc)"; [done|apply proph_dep_constr, proph_dep_one|done|].
+    iCombine "Obs Obs'" as "Obs". iSpecialize ("ζPc" with "ζ").
+    iExists ((λ π, (aπ π, π ζ)) -:: _). iFrame "T".
+    iMod ("ToBor" with "[ToξPc] [↦ty ζPc]") as "[Bor κ]"; last first.
+    - iMod ("ToL" with "κ") as "$". iModIntro. iSplitR "Obs"; last first.
+      { iApply proph_obs_impl; [|done]=>/= π. move: (equal_f Eq π).
+        rewrite /aπ /=. case (vπ π)=>/= ??<-[? /(f_equal g) +].
+        have ->: ∀x, g (f x) = (g ∘ f) x by done. rewrite semi_iso. by move=>/= <-. }
+      iExists _, _. iSplit; [done|]. iFrame "⧖ In". iExists _, _. by iFrame.
+    - iNext. iExists _, _. iFrame "⧖ ζPc".
+      iDestruct "↦ty" as (?) "[↦ (%& %Eq' & ty)]". iExists _. iFrame "↦".
+      by rewrite /aπ -compose_assoc Eq' compose_assoc semi_iso.
+    - iIntros "!> (%&%& ↦ty & ⧖' & ζPc) !>!>". iExists _, _.
+      iFrame "⧖'". iSplitL "↦ty"; last first. { iApply "ToξPc".
+      iApply proph_eqz_constr. by iApply proph_ctrl_eqz. }
+      iDestruct "↦ty" as (?) "[↦ ty]". iExists _. iFrame "↦". iExists _. by iFrame.
   Qed.
 
 End typing.
